Griotte: deep locality and deep immutability (#2)
* WIP add DL and DRO

* WIP add DL and DRO

* WIP add DL and DRO --- FTLR except load

* WIP

* Update logrel for E and sealed to support borrowing + WIP proof FTLR load

* WIP

* Fix V(E,g,---) to include E(RX,g,--) and E(RX,Local,--) + finish proof FTLR

theories/ftlr/Load.v
@@ -30,14 +30,13 @@ Section fundamental.
   (* The necessary resources to close the region again,
      except for the points to predicate, which we will store separately
      The boolean bl can be used to keep track of whether or not we have applied a wp lemma *)
-  Definition region_open_resources W l ls p φ v (has_later : bool): iProp Σ :=
+  Definition region_open_resources W a als p φ v (has_later : bool): iProp Σ :=
     (∃ ρ,
-     sts_state_std l ρ
+     sts_state_std a ρ
     ∗ ⌜ρ ≠ Revoked ∧ (∀ g, ρ ≠ Frozen g)⌝
-    ∗ open_region_many (l :: ls) W
-    ∗ if_later_P has_later (monotonicity_guarantees_region ρ v p φ
-                  ∗ φ (W, v))
-    ∗ rel l p φ)%I.
+    ∗ open_region_many (a :: als) W
+    ∗ if_later_P has_later (monotonicity_guarantees_region ρ v p φ ∗ φ (W, v))
+    ∗ rel a p φ)%I.
 
   Lemma load_inr_eq {regs r p0 g0 b0 e0 a0 p1 g1 b1 e1 a1}:
     reg_allows_load regs r p0 g0 b0 e0 a0 →
@@ -52,46 +51,75 @@ Section fundamental.
   (* Description of what the resources are supposed to look like
      after opening the region if we need to,
      but before closing the region up again*)
-  Definition allow_load_res W r (regs : Reg) pc_a:=
+  Definition allow_load_res W r (regs : Reg) pc_a pc_p :=
     (∃ p g b e a, ⌜read_reg_inr regs r p g b e a⌝ ∗
-    if decide (reg_allows_load regs r p g b e a ∧ a ≠ pc_a )
-    then ∃ w p' (P:D),
-        ⌜p' ≠ O⌝
-        ∗ ⌜(∀ Wv, Persistent (P Wv.1 Wv.2))⌝
-        ∗ a ↦ₐ w
-        ∗ (region_open_resources W a [pc_a] p' (λ Wv, P Wv.1 Wv.2) w true)
-        ∗ ▷ rcond P interp
+    if decide (reg_allows_load regs r p g b e a)
+    then (if decide (a ≠ pc_a)
+          then ∃ w p' (P:D),
+              ⌜PermFlowsTo p p'⌝
+              ∗ ⌜(∀ Wv, Persistent (P Wv.1 Wv.2))⌝
+              ∗ a ↦ₐ w
+              ∗ (region_open_resources W a [pc_a] p' (λ Wv, P Wv.1 Wv.2) w true)
+              ∗ ▷ rcond p' P interp
+          else open_region pc_a W ∗ ⌜PermFlowsTo p pc_p⌝)
     else open_region pc_a W)%I.
 
-  Definition allow_load_mem W r (regs : Reg) pc_a pc_w (mem : Mem) (has_later: bool):=
-    (∃ p g b e a, ⌜read_reg_inr regs r p g b e a⌝ ∗
-    if decide (reg_allows_load regs r p g b e a ∧ a ≠ pc_a)
-    then ∃ w p' (P:D),
-        ⌜p' ≠ O⌝
-        ∗ ⌜(∀ Wv, Persistent (P Wv.1 Wv.2))⌝
-        ∗ ⌜mem = <[a:=w]> (<[pc_a:=pc_w]> ∅)⌝
-        ∗ (region_open_resources W a [pc_a] p' (λ Wv, P Wv.1 Wv.2) w has_later)
-        ∗ if_later_P has_later (rcond P interp)
-    else  ⌜mem = <[pc_a:=pc_w]> ∅⌝ ∗ open_region pc_a W)%I.
-
-  Lemma create_load_res:
-    ∀ (W : WORLD) (regs : leibnizO Reg)
-      (p : Perm) (g : Locality) (b e a : Addr)
-      (src : RegName)
-      (p0 : Perm) (g0 : Locality) (b0 e0 a0 : Addr),
-      read_reg_inr (<[PC:=WCap p g b e a]> regs) src p0 g0 b0 e0 a0
-      → (∀ (r : RegName) (v : Word), ⌜r ≠ PC⌝ → ⌜regs !! r = Some v⌝ → ((fixpoint interp1) W) v)
-          -∗ open_region a W
-          -∗ sts_full_world W
-          -∗ allow_load_res W src (<[PC:= WCap p g b e a]> regs) a
-          ∗ sts_full_world W.
+   Lemma interp_hpf_eq (W : WORLD) P (regs : leibnizO Reg) (r1 : RegName)
+    p g b e a pc_p pc_g pc_b pc_e pc_p' :
+    reg_allows_load (<[PC:=WCap pc_p pc_g pc_b pc_e a]> regs) r1 p g b e a
+    → PermFlowsTo pc_p pc_p'
+    → (∀ (r1 : RegName) v, ⌜r1 ≠ PC⌝ → ⌜regs !! r1 = Some v⌝ → ((fixpoint interp1) W) v)
+    -∗ rel a pc_p' P
+    -∗ ⌜PermFlowsTo p pc_p'⌝.
   Proof.
-    intros W regs p g b e a src p0 g0 b0 e0 a0 HVsrc.
-    iIntros "#Hreg Hr Hsts".
+    destruct (decide (r1 = PC)).
+    - subst r1. iIntros ([? ?] ?). simplify_map_eq; auto.
+    - iIntros ((Hsomer1 & Hwa & Hwb) Hfl) "Hreg #Hinva".
+      simplify_map_eq.
+      iDestruct ("Hreg" $! r1 _ n Hsomer1) as "Hr1"; eauto.
+      iDestruct (read_allowed_inv _ a with "Hr1")
+        as (p'' P'' Hflp'' Hcond_pers'') "(Hrel'' & Hzcond'' & Hrcond'' & Hwcond'')"; auto.
+      { apply andb_true_iff in Hwb as [Hle Hge].
+        split; [apply Zle_is_le_bool | apply Zlt_is_lt_bool]; auto. }
+      iDestruct (rel_agree a _ _ p'' pc_p' with "[$Hinva $Hrel'']") as "[-> _]".
+      done.
+  Qed.
+
+  Definition allow_load_mem W r (regs : Reg) pc_a pc_p pc_w (mem : Mem) (has_later: bool):=
+    (∃ p g b e a, ⌜read_reg_inr regs r p g b e a⌝ ∗
+    if decide (reg_allows_load regs r p g b e a)
+    then (if decide (a ≠ pc_a)
+          then ∃ w p' (P:D),
+              ⌜PermFlowsTo p p'⌝
+              ∗ ⌜(∀ Wv, Persistent (P Wv.1 Wv.2))⌝
+              ∗ ⌜mem = <[a:=w]> (<[pc_a:=pc_w]> ∅)⌝
+              ∗ (region_open_resources W a [pc_a] p' (λ Wv, P Wv.1 Wv.2) w has_later)
+              ∗ if_later_P has_later (rcond p' P interp)
+          else ⌜mem = <[pc_a:=pc_w]> ∅⌝ ∗ open_region pc_a W ∗ ⌜PermFlowsTo p pc_p⌝ )
+    else ⌜mem = <[pc_a:=pc_w]> ∅⌝ ∗ open_region pc_a W)%I.
+
+  Lemma create_load_res
+    (W : WORLD) (regs : leibnizO Reg)
+    (p_pc p_pc' : Perm) (g_pc : Locality) (b_pc e_pc a_pc : Addr)
+    (src : RegName)
+    (p : Perm) (g : Locality) (b e a : Addr) (P:D):
+    read_reg_inr (<[PC:=WCap p_pc g_pc b_pc e_pc a_pc]> regs) src p g b e a
+    → PermFlowsTo p_pc p_pc'
+    → (∀ (r : RegName) (v : Word), ⌜r ≠ PC⌝ → ⌜regs !! r = Some v⌝ → interp W v)
+    -∗ rel a_pc p_pc' (safeC P)
+    -∗ open_region a_pc W
+    -∗ sts_full_world W
+    -∗ (allow_load_res W src (<[PC:= WCap p_pc g_pc b_pc e_pc a_pc]> regs) a_pc p_pc'
+        ∗ sts_full_world W).
+  Proof.
+    iIntros (HVsrc Hfl) "#Hreg #Hinva Hr Hsts".
     do 5 (iApply sep_exist_r; iExists _). iFrame "%".
-    case_decide as Hdec; last iFrame.
-    destruct Hdec as [Hallows Haeq].
-    destruct Hallows as [Hrinr [Hra Hwb] ].
+    case_decide as Hallows; last by iFrame.
+    case_decide as Haeq ; cycle 1.
+    { simplify_eq; iFrame.
+      iApply interp_hpf_eq; eauto.
+    }
+    destruct Hallows as (Hrinr & Hra & Hwb).
     apply andb_prop in Hwb as [Hle Hge].
 
     (* Unlike in the old proof, we now go the other way around,
@@ -102,147 +130,198 @@ Section fundamental.
     simplify_map_eq.
 
     iDestruct ("Hreg" $! src _ n Hrinr) as "Hvsrc"; eauto.
-    iDestruct (read_allowed_inv _ a0 with "Hvsrc")
-      as (p' P Hflp' Hcond_pers) "(Hrel & Hzcond & Hrcond & Hwcond)"; auto
+    iDestruct (read_allowed_inv _ a with "Hvsrc")
+      as (p0 P0 Hflp0 Hcond_pers0) "(Hrel0 & Hzcond0 & Hrcond0 & Hwcond0)"; auto
     ; first (split; [by apply Z.leb_le | by apply Z.ltb_lt]).
 
     iDestruct (region_open_prepare with "Hr") as "Hr".
     iDestruct (readAllowed_valid_cap_implies with "Hvsrc") as %HH; eauto.
     { rewrite /withinBounds Hle Hge. auto. }
-    destruct HH as [ρ' [Hstd [Hnotrevoked' Hnotfrozen' ] ] ].
+    destruct HH as (ρ0 & Hstd & Hnotrevoked0 & Hnotfrozen0).
     (* We can finally frame off Hsts here,
             since it is no longer needed after opening the region*)
-    iDestruct (region_open_next _ _ _ a0 p' ρ' with "[$Hrel $Hr $Hsts]")
+    iDestruct (region_open_next _ _ _ a p0 ρ0 with "[$Hrel0 $Hr $Hsts]")
       as (w0) "($ & Hstate' & Hr & Ha0 & Hfuture & Hval)"; eauto.
-    { intros [m' Hcontr]. specialize (Hnotfrozen' m'); contradiction. }
+    { intros [m' Hcontr]. specialize (Hnotfrozen0 m'); contradiction. }
     { apply not_elem_of_cons. split; auto. apply not_elem_of_nil. }
-    iExists w0,p',P.
-    iFrame "∗#".
-    iSplitR;[iPureIntro ; destruct_perm p0; destruct_perm p'; done|].
-    rewrite /persistent_cond in Hcond_pers.
+    iExists w0,p0,P0.
+    iFrame "∗#%".
     iSplitR; iPureIntro;done.
   Qed.
 
-  Lemma load_res_implies_mem_map:
-    ∀ (W : WORLD) (regs : leibnizO Reg)
-      (a : Addr) (w : Word) (src : RegName),
-    allow_load_res W src regs a
+  Lemma load_res_implies_mem_map
+    (W : WORLD) (regs : leibnizO Reg)
+      (p : Perm) (a : Addr) (w : Word) (src : RegName):
+    allow_load_res W src regs a p
     -∗ a ↦ₐ w
     -∗ ∃ mem0 : Mem,
-        allow_load_mem W src regs a w mem0 true
+        allow_load_mem W src regs a p w mem0 true
         ∗ ▷ ([∗ map] a0↦w ∈ mem0, a0 ↦ₐ w).
   Proof.
-    intros W regs a w src.
     iIntros "HLoadRes Ha".
     iDestruct "HLoadRes" as (p1 g1 b1 e1 a1) "[% HLoadRes]".
-
-    case_decide as Hdec. 1: destruct Hdec as [ Hallows Haeq ].
-    -  pose(Hallows' := Hallows). destruct Hallows' as [Hrinr [Hra Hwb] ].
-       iDestruct "HLoadRes" as (w0 p' P Hp'O Hpers) "[HLoadCh [HLoadRest #Hrcond] ]".
-       iExists _.
-       iSplitL "HLoadRest".
-       + iExists p1,g1,b1,e1,a1. iSplitR; first auto.
-         case_decide as Hdec1.
-         2: apply not_and_r in Hdec1 as [|]; by exfalso.
-         iExists w0,p',P.
-         repeat (iSplit; auto).
-       + iNext.
-         iApply memMap_resource_2ne; auto; iFrame.
-    - iExists _.
+    case_decide as Hallows; cycle 1.
+    {
+      iExists _.
       iSplitL "HLoadRes".
       + iExists p1,g1,b1,e1,a1. iSplitR; auto.
         case_decide; first by exfalso. auto.
       + iNext. by iApply memMap_resource_1.
+    }
+    case_decide as Haeq.
+    - pose(Hallows' := Hallows).
+      destruct Hallows' as (Hrinr & Hra & Hwb).
+      iDestruct "HLoadRes" as (w0 p' P Hp'O Hpers) "[HLoadCh [HLoadRest #Hrcond] ]".
+      iExists _.
+      iSplitL "HLoadRest".
+      + iExists p1,g1,b1,e1,a1. iFrame "%".
+        case_decide; last by exfalso.
+        case_decide; last by exfalso.
+        iExists w0,p',P.
+        repeat (iSplit; auto).
+      + iNext.
+        iApply memMap_resource_2ne; auto; iFrame.
+    - iExists _.
+      iSplitL "HLoadRes"; last (iNext; by iApply memMap_resource_1).
+      iExists p1,g1,b1,e1,a1. iFrame "%".
+      case_decide; last by exfalso.
+      case_decide; first by exfalso.
+      by iFrame.
   Qed.
 
-  Lemma mem_map_implies_pure_conds:
-    ∀ (W : WORLD) (regs : leibnizO Reg)
-      (a : Addr) (w : Word) (src : RegName)
-      (mem0 : Mem),
-    allow_load_mem W src regs a w mem0 true
+  Lemma mem_map_implies_pure_conds
+    (W : WORLD) (regs : leibnizO Reg)
+      (p : Perm) (a : Addr) (w : Word) (src : RegName)
+      (mem0 : Mem):
+    allow_load_mem W src regs a p w mem0 true
     -∗ ⌜mem0 !! a = Some w⌝ ∗ ⌜allow_load_map_or_true src regs mem0⌝.
   Proof.
-    iIntros (W regs a w src mem0) "HLoadMem".
+    iIntros "HLoadMem".
     iDestruct "HLoadMem" as (p1 g1 b1 e1 a1) "[% HLoadRes]".
-    case_decide as Hdec. 1: destruct Hdec as [ Hallows Haeq ].
-    -  pose(Hallows' := Hallows). destruct Hallows' as [Hrinr [Hra Hwb] ].
-       (* case_decide as Haeq. *)
-       iDestruct "HLoadRes" as (w0 p' P Hp'O Hpers) "[-> _]".
-       iSplitR. rewrite lookup_insert_ne; auto. by rewrite lookup_insert.
-       iExists p1,g1,b1,e1,a1. iSplitR; auto.
-       case_decide; last by exfalso.
-       iExists w0.
-       by rewrite lookup_insert.
-    - iDestruct "HLoadRes" as "[-> HLoadRes ]".
+    case_decide as Hallows; cycle 1.
+    {
+      iDestruct "HLoadRes" as "[-> HLoadRes ]".
       iSplitR. by rewrite lookup_insert.
       iExists p1,g1,b1,e1,a1. iSplitR; auto.
       case_decide as Hdec1; last by done.
-      apply not_and_r in Hdec as [| <-%dec_stable]; first by exfalso.
+      done.
+    }
+
+    case_decide as Haeq.
+    - pose(Hallows' := Hallows).
+      destruct Hallows' as (Hrinr & Hra & Hwb).
+      (* case_decide as Haeq. *)
+      iDestruct "HLoadRes" as (w0 p' P Hp'O Hpers) "[-> _]".
+      iSplitR. rewrite lookup_insert_ne; auto. by rewrite lookup_insert.
+      iExists p1,g1,b1,e1,a1. iSplitR; auto.
+      case_decide; last by exfalso.
+      iExists w0.
+      by rewrite lookup_insert.
+    - subst a. iDestruct "HLoadRes" as "[-> HLoadRes]".
+      iSplitR. by rewrite lookup_insert.
+      iExists p1,g1,b1,e1,a1. repeat iSplitR; auto.
+      case_decide as Hdec1; last by done.
       iExists w. by rewrite lookup_insert.
   Qed.
 
-  Lemma allow_load_mem_later:
-    ∀ (W : WORLD) (regs : leibnizO Reg)
-      (p : Perm) (g : Locality) (b e a : Addr)
-      (w : Word) (src : RegName) (mem0 : Mem),
-    allow_load_mem W src regs a w mem0 true
-    -∗ ▷ allow_load_mem W src regs a w mem0 false.
+  Lemma allow_load_mem_later
+    (W : WORLD) (regs : leibnizO Reg)
+    (p : Perm) (g : Locality) (b e a : Addr)
+    (w : Word) (src : RegName) (mem0 : Mem):
+    allow_load_mem W src regs a p w mem0 true
+    -∗ ▷ allow_load_mem W src regs a p w mem0 false.
   Proof.
-    iIntros (W regs p g b e a w src mem0) "HLoadMem".
+    iIntros "HLoadMem".
     iDestruct "HLoadMem" as (p0 g0 b0 e0 a0) "[% HLoadMem]".
     do 5 (iApply later_exist_2; iExists _). iApply later_sep_2; iSplitR; auto.
+    case_decide; last iFrame.
     case_decide; last iFrame.
     iDestruct "HLoadMem" as (w0 p' P Hp'O Hpers) "(-> & HLoadMem & #Hrcond)".
     do 3 (iApply later_exist_2; iExists _).
     do 2 (iApply later_sep_2; iSplitR; auto).
   Qed.
 
-  Lemma mem_map_recover_res:
-    ∀ (W : WORLD) (regs : leibnizO Reg)
-      (a : Addr) (w : Word) (src : RegName)
-      (p0 : Perm) (g0 : Locality) (b0 e0 a0 : Addr)
-      (mem0 : Mem) (loadv : Word),
-    reg_allows_load regs src p0 g0 b0 e0 a0
-    → mem0 !! a0 = Some loadv
-    → allow_load_mem W src regs a w mem0 false
-    -∗ ((fixpoint interp1) W) w
-    -∗ ([∗ map] a0↦w ∈ mem0, a0 ↦ₐ w)
-    -∗ open_region a W ∗ a ↦ₐ w ∗ ((fixpoint interp1) W) loadv.
+  Definition rcond' (P : D) p g b e a regs p' : iProp Σ
+    := (if decide (readAllowed_in_r_a (<[PC:=WCap p g b e a]> regs) a)
+             then (rcond p' P interp)
+             else emp)%I.
+  Instance rcond'_pers P p g b e a regs p' : Persistent (rcond' P p g b e a regs p' ).
+  Proof. intros. rewrite /rcond'. case_decide;apply _. Qed.
+
+  Lemma mem_map_recover_res
+    (W : WORLD) (regs : leibnizO Reg)
+    (pc_w : Word) (src : RegName)
+    (p_pc p_pc' : Perm) (g_pc : Locality) (b_pc e_pc a_pc : Addr)
+    (p : Perm) (g : Locality) (b e a : Addr)
+    (mem0 : Mem) (loadv : Word) (P:D) :
+    PermFlowsTo p_pc p_pc'
+    -> reg_allows_load (<[PC:=WCap p_pc g_pc b_pc e_pc a_pc]> regs) src p g b e a
+    -> mem0 !! a = Some loadv
+    -> interp W (WCap p_pc g_pc b_pc e_pc a_pc)
+      -∗ (∀ r v, ⌜r ≠ PC⌝ → ⌜regs !! r = Some v⌝ → fixpoint interp1 W v)
+         -∗ rcond' P p_pc g_pc b_pc e_pc a_pc regs p_pc'
+            -∗ P W pc_w
+               -∗ ([∗ map] a1↦w0 ∈ mem0, a1 ↦ₐ w0)
+                  -∗ allow_load_mem W src (<[PC:=WCap p_pc g_pc b_pc e_pc a_pc]> regs) a_pc p_pc' pc_w mem0 false
+                     -∗ open_region a_pc W ∗ a_pc ↦ₐ pc_w ∗ interp W (load_word p loadv).
   Proof.
-    intros W regs a w src p0 g0 b0 e0 a0 mem0 loadv Hrar Ha0.
-    iIntros "HLoadMem #Hw Hmem".
+    intros Hflpc Hrar Ha.
+    iIntros "##Hinterp_pc Hreg #Hrcond Hw Hmem HLoadMem".
     iDestruct "HLoadMem" as (p1 g1 b1 e1 a1) "[%Hread HLoadRes]".
     destruct (load_inr_eq Hrar Hread) as (<- & <- & <- & <- & <-).
-    case_decide as Hdec. destruct Hdec as [Hallows Heq].
-    -  destruct Hallows as [Hrinr [Hra Hwb] ].
-       iDestruct "HLoadRes" as (w0 p' P Hp'O Hpers) "(-> & HLoadRes & #Hrcond)".
-       iDestruct "HLoadRes" as (ρ1) "(Hstate' & #Hrev & Hr & (Hfuture & #HV) & Hrel')".
-       iDestruct "Hrev" as %[Hnotrevoked Hnotfrozen ].
-       rewrite memMap_resource_2ne; last auto. iDestruct "Hmem" as  "[Ha1 $]".
-       iDestruct (region_close_next with "[$Hr $Ha1 $Hrel' $Hstate' $Hfuture]")
-         as "Hr"; eauto.
-       { intros [m' Hm']; specialize (Hnotfrozen m'); contradiction. }
-       { apply not_elem_of_cons; split; [auto|apply not_elem_of_nil]. }
-       iDestruct (region_open_prepare with "Hr") as "$".
-       simplify_map_eq.
-       iApply "Hrcond". simpl. iFrame "#".
-    - apply not_and_r in Hdec as [| <-%dec_stable].
-      * by exfalso.
-      * iDestruct "HLoadRes" as "[-> $ ]".
-        rewrite -memMap_resource_1.
-        rewrite lookup_insert in Ha0. inversion Ha0. by iFrame.
+    case_decide as Hallows; last by exfalso.
+    destruct Hallows as (Hrinr & Hwa & Hwb).
+    case_decide as Haeq; cycle 1.
+    - iDestruct "HLoadRes" as "(-> & $ & %Hfl')".
+      simplify_map_eq.
+      rewrite -memMap_resource_1.
+      iFrame.
+      rewrite /rcond'.
+      rewrite decide_True.
+      2: { eexists src,_.
+           inversion Hrar.
+           split. eauto.
+           split;auto.
+           split;auto.
+           destruct H0.
+           apply withinBounds_le_addr in H1; auto.
+      }
+      iApply interp_weakening_word_load; eauto.
+      by iApply "Hrcond".
+    - iDestruct "HLoadRes"
+        as (w p' P' Hflp'' HpersP') "(-> & HLoadRes & #Hrcond')".
+      rewrite lookup_insert in Ha; inversion Ha; clear Ha; subst.
+      rewrite memMap_resource_2ne; last auto.
+      iDestruct "Hmem" as "[Ha Hapc]"; iFrame.
+      iDestruct "HLoadRes" as (ρ1) "(Hstate' & [%Hnotrevoked %Hnotfrozen] & Hr & (Hfuture & #HV) & Hrel')"
+      ; cbn.
+
+      assert (isO p' = false) as HpO'.
+      { eapply readAllowed_flows in Hflp''; auto.
+        eapply readAllowed_nonO in Hflp''; eauto.
+        reflexivity.
+      }
+      iDestruct (region_close_next with "[$Hr $Ha $Hrel' $Hstate' $Hfuture]")
+        as "Hr"; eauto.
+      { intros [m' Hm']; specialize (Hnotfrozen m'); contradiction. }
+      { apply not_elem_of_cons; split; [auto|apply not_elem_of_nil]. }
+      iFrame.
+      iDestruct (region_open_prepare with "Hr") as "$".
+      iDestruct ("Hrcond'" with "HV") as "HV'".
+      iApply interp_weakening_word_load; eauto.
   Qed.
 
-
-   Lemma load_case (W : WORLD) (regs : leibnizO Reg)
-     (p p' : Perm) (g : Locality) (b e a : Addr)
-     (w : Word) (ρ : region_type) (dst src : RegName) (P:D) :
+  Lemma load_case (W : WORLD) (regs : leibnizO Reg)
+    (p p' : Perm) (g : Locality) (b e a : Addr)
+    (w : Word) (ρ : region_type) (dst src : RegName) (P:D) :
     ftlr_instr W regs p p' g b e a w (Load dst src) ρ P.
   Proof.
-    intros Hp Hsome i Hbae Hfp HO Hpers Hpwl Hregion Hnotrevoked Hnotfrozen Hi.
+    intros Hp Hsome HcorrectPC Hbae Hfp HO Hpers Hpwl Hregion Hnotrevoked Hnotfrozen Hi.
     iIntros "#IH #Hinv_interp #Hreg #Hinva #Hrcond #Hwcond #Hmono #HmonoV Hw Hsts Hown".
     iIntros "Hr Hstate Ha HPC Hmap".
     iInsert "Hmap" PC.
+    iClear "Hwcond".
+    iDestruct (if_dec_later with "Hrcond") as "Hrcond'"; iClear "Hrcond".
 
     assert (Persistent (▷ P W w)) as HpersP.
     { apply later_persistent. specialize (Hpers (W,w)). auto. }
@@ -269,7 +348,7 @@ Section fundamental.
     }
 
     (* Step 1: open the region, if necessary, and store all the resources obtained from the region in allow_load_res *)
-    iDestruct (create_load_res with "Hreg Hr Hsts") as "[HLoadRes Hsts]"; eauto.
+    iDestruct (create_load_res with "Hreg Hinva Hr Hsts") as "[HLoadRes Hsts]"; eauto.
     (* Clear helper values; they exist in the existential now *)
     clear HVsrc p0 g0 b0 e0 a0.
 
@@ -289,19 +368,18 @@ Section fundamental.
     { iSplitR "Hmap"; auto. }
     iNext. iIntros (regs' retv). iDestruct 1 as (HSpec) "[Hmem Hmap]".
 
-    destruct HSpec as [* ? ? Hincr|].
+    destruct HSpec as [ * Hreg_load Hmem_a Hincr|].
     { apply incrementPC_Some_inv in Hincr.
       destruct Hincr as (?&?&?&?&?&?&?&?&XX).
       iApply wp_pure_step_later; auto. iNext; iIntros "_".
 
       (* Step 5: return all the resources we had in order to close the second location in the region, in the cases where we need to *)
-      iDestruct (mem_map_recover_res with "HLoadMem [] Hmem") as "[Hr [Ha #HLVInterp ] ]"; eauto.
-      { by iApply "Hrcond". }
+      iDestruct (mem_map_recover_res with "Hinv_interp Hreg Hrcond' Hw Hmem HLoadMem") as
+        "[Hr [Ha #HLVInterp ] ]"; eauto.
 
       (* Exceptional success case: we do not apply the induction hypothesis in case we have a faulty PC*)
-      destruct (decide (x = RX ∨ x = RWX ∨ x = RWLX)) as [Hp'|Hp'].
+      destruct (executeAllowed x) eqn:Hp'.
       2 : {
-        assert (x ≠ RX ∧ x ≠ RWX ∧ x ≠ RWLX). split; last split; by auto.
         iDestruct ((big_sepM_delete _ _ PC) with "Hmap") as "[HPC Hmap]".
         { subst. by rewrite lookup_insert. }
         iApply (wp_bind (fill [SeqCtx])).
@@ -310,8 +388,8 @@ Section fundamental.
         iIntros (a1); inversion a1.
       }
 
-      iDestruct (region_close with "[$Hstate $Hr $Ha $HmonoV]") as "Hr"; eauto.
-      { destruct ρ;auto;[|specialize (Hnotfrozen g1)];contradiction. }
+      iDestruct (region_close with "[$Hstate $Ha $Hr $HmonoV]") as "Hr"; eauto.
+      { destruct ρ;auto;[|ospecialize (Hnotfrozen _)];contradiction. }
       iApply ("IH" $! _ regs' with "[%] [] [Hmap] [$Hr] [$Hsts] [$Hown]").
       { cbn. intros. subst regs'.
         rewrite lookup_insert_is_Some.
@@ -327,20 +405,12 @@ Section fundamental.
         { simplify_map_eq; iApply "Hreg"; auto. }
        }
        { subst regs'. rewrite insert_insert. iApply "Hmap". }
-       { destruct (decide (PC = dst)); simplify_eq.
-         - destruct Hp' as [HRX | [HRWX | HRWLX] ]; auto.
-           subst; simplify_map_eq.
-           iDestruct (writeLocalAllowed_implies_local _ RWLX with "[HLVInterp]") as "%"; auto.
-           destruct x0; unfold isLocal in *.
-           all: try done.
-           iPureIntro; do 2 right; auto; simplify_map_eq.
-         - simplify_map_eq; iPureIntro; naive_solver.
-       }
        {
         destruct (decide (PC = dst)); simplify_map_eq; cycle 1.
-        iApply (interp_next_PC with "IH Hinv_interp"); eauto.
-        iApply (interp_weakening with "IH HLVInterp"); eauto; try solve_addr; try done.
-        naive_solver.
+        + iApply (interp_next_PC with "Hinv_interp"); eauto.
+        + rewrite H.
+          iApply (interp_weakening with "IH HLVInterp"); eauto; try solve_addr; try done.
+          by apply executeAllowed_isnot_sentry.
        }
     }
     { iApply wp_pure_step_later; auto.
