theories/logrel.v
@@ -119,13 +119,13 @@ Program Definition interp_expr (interp : D) r : D :=
     Contractive (λ interp, ▷ zcond P)%I.
   Proof. solve_contractive. Qed.
 
-  Definition rcond (P interp : D) : iProp Σ :=
-    (□ ∀ (W: WORLD) (w : Word), P W w -∗ interp W w).
+  Definition rcond (p : Perm) (P interp : D) : iProp Σ :=
+    (□ ∀ (W: WORLD) (w : Word), P W w -∗ interp W (load_word p w)).
   Global Instance rcond_ne n :
-    Proper ((=) ==> dist n ==> dist n) rcond.
+    Proper ((=) ==> (=) ==> dist n ==> dist n) rcond.
   Proof. solve_proper_prepare. repeat f_equiv;auto. Qed.
-  Global Instance rcond_contractive P :
-    Contractive (λ interp, ▷ rcond P interp)%I.
+  Global Instance rcond_contractive p P :
+    Contractive (λ interp, ▷ rcond p P interp)%I.
   Proof. solve_contractive. Qed.
 
   Definition wcond (P interp : D) : iProp Σ :=
@@ -150,7 +150,9 @@ Program Definition interp_expr (interp : D) r : D :=
 
   Definition enter_cond W p g b e a (interp : D) : iProp Σ :=
     (∀ r W', future_world g W W' →
-        ▷ interp_expr interp r W' (WCap p g b e a))%I.
+             (▷ interp_expr interp r W' (WCap p g b e a))
+               ∗ (▷ interp_expr interp r W' (WCap p Local b e a))
+    )%I.
   Global Instance enter_cond_ne n :
     Proper ((=) ==> (=) ==> (=) ==> (=) ==> (=) ==> (=) ==> dist n ==> dist n) enter_cond.
   Proof. unfold enter_cond. solve_proper. Qed.
@@ -188,17 +190,6 @@ Program Definition interp_expr (interp : D) r : D :=
   (* For simplicity we might want to have the following statement in valididy of caps.
      However, it is strictly not necessary since it can be derived form full_sts_world *)
 
-  Definition interp_z : D := λne _ w, ⌜match w with WInt z => True | _ => False end⌝%I.
-  Definition interp_cap_O : D := λne _ _, True%I.
-
-  Program Definition interp_cap_E (interp : D) : D :=
-    λne W w, (match w with
-              | WCap E g b e a =>
-                  □ enter_cond W RX g b e a interp
-              | _ => False
-              end)%I.
-  Solve All Obligations with solve_proper.
-
   Definition safeC (P : D) :=
     (λ Wv : WORLD * (leibnizO Word), (P Wv.1) Wv.2).
 
@@ -212,141 +203,36 @@ Program Definition interp_expr (interp : D) r : D :=
     | _ => True%I
     end.
 
-  Program Definition interp_cap_WO (interp : D) : D :=
+  Definition interp_z : D := λne _ w, ⌜match w with WInt z => True | _ => False end⌝%I.
+  Definition interp_cap_O : D := λne _ _, True%I.
+
+  Program Definition interp_cap_E (interp : D) : D :=
     λne W w, (match w with
-              | WCap WO g b e a =>
-                  [∗ list] a ∈ (finz.seq_between b e),
-                    ∃ (p' : Perm) (P:D),
-                      ⌜PermFlowsTo WO p'⌝
-                      ∧ ⌜persistent_cond P⌝
-                      ∧ rel a p' (λne Wv, P Wv.1 Wv.2)
-                      ∧ ▷ zcond P
-                      ∧ (if readAllowed p' then ▷ rcond P interp else True)
-                      ∧ (if writeAllowed p' then ▷ wcond P interp else True)
-                      ∧ monoReq W a p' P
-                      ∧ ⌜ region_state_nwl W a g ⌝
+              | WCap E g b e a => (□ enter_cond W RX g b e a interp)
               | _ => False
               end)%I.
   Solve All Obligations with solve_proper.
 
-  Program Definition interp_cap_WLO (interp : D) : D :=
+  Program Definition interp_cap (interp : D) : D :=
     λne W w, (match w with
-              | WCap WLO Local b e a =>
+              | WCap E _ _ _ _
+              | WCap (O _ _) _ _ _ _
+              | WCap (BPerm _ WL _ _) Global _ _ _ => False
+              | WCap p g b e a =>
                   [∗ list] a ∈ (finz.seq_between b e),
                     ∃ (p' : Perm) (P:D),
-                      ⌜PermFlowsTo WLO p'⌝
+                      ⌜PermFlowsTo p p'⌝
                       ∧ ⌜persistent_cond P⌝
                       ∧ rel a p' (λne Wv, P Wv.1 Wv.2)
                       ∧ ▷ zcond P
-                      ∧ (if readAllowed p' then ▷ rcond P interp else True)
+                      ∧ (if readAllowed p' then ▷ rcond p' P interp else True)
                       ∧ (if writeAllowed p' then ▷ wcond P interp else True)
                       ∧ monoReq W a p' P
-                      ∧ ⌜ region_state_pwl W a ⌝
+                      ∧ ⌜ if pwl p then region_state_pwl W a else region_state_nwl W a g⌝
               | _ => False
               end)%I.
-  Solve All Obligations with solve_proper.
+  Solve All Obligations with auto;solve_proper.
 
-  Program Definition interp_cap_RO (interp : D) : D :=
-    λne W w, (match w with
-              | WCap RO g b e a =>
-                  [∗ list] a ∈ (finz.seq_between b e),
-                    ∃ (p' : Perm) (P:D),
-                      ⌜PermFlowsTo RO p'⌝
-                      ∧ ⌜persistent_cond P⌝
-                      ∧ rel a p' (λne Wv, P Wv.1 Wv.2)
-                      ∧ ▷ zcond P
-                      ∧ (if readAllowed p' then ▷ rcond P interp else True)
-                      ∧ (if writeAllowed p' then ▷ wcond P interp else True)
-                      ∧ monoReq W a p' P
-                      ∧ ⌜ region_state_nwl W a g ⌝
-              | _ => False
-              end)%I.
-  Solve All Obligations with solve_proper.
-
-  Program Definition interp_cap_RW (interp : D) : D :=
-    λne W w, (match w with
-              | WCap RW g b e a =>
-                  [∗ list] a ∈ (finz.seq_between b e),
-                    ∃ (p' : Perm) (P:D),
-                      ⌜PermFlowsTo RW p'⌝
-                      ∧ ⌜persistent_cond P⌝
-                      ∧ rel a p' (λne Wv, P Wv.1 Wv.2)
-                      ∧ ▷ zcond P
-                      ∧ (if readAllowed p' then ▷ rcond P interp else True)
-                      ∧ (if writeAllowed p' then ▷ wcond P interp else True)
-                      ∧ monoReq W a p' P
-                      ∧ ⌜ region_state_nwl W a g ⌝
-              | _ => False
-              end)%I.
-  Solve All Obligations with solve_proper.
-
-  Program Definition interp_cap_RWL (interp : D) : D :=
-    λne W w, (match w with
-              | WCap RWL Local b e a =>
-                  [∗ list] a ∈ (finz.seq_between b e),
-                    ∃ (p' : Perm) (P:D),
-                      ⌜PermFlowsTo RWL p'⌝
-                      ∧ ⌜persistent_cond P⌝
-                      ∧ rel a p' (λne Wv, P Wv.1 Wv.2)
-                      ∧ ▷ zcond P
-                      ∧ (if readAllowed p' then ▷ rcond P interp else True)
-                      ∧ (if writeAllowed p' then ▷ wcond P interp else True)
-                      ∧ monoReq W a p' P
-                      ∧ ⌜ region_state_pwl W a ⌝
-              | _ => False
-              end)%I.
-  Solve All Obligations with solve_proper.
-
-  Program Definition interp_cap_RX (interp : D) : D :=
-    λne W w, (match w with
-              | WCap RX g b e a =>
-                  [∗ list] a ∈ (finz.seq_between b e),
-                    ∃ (p' : Perm) (P:D),
-                      ⌜PermFlowsTo RX p'⌝
-                      ∧ ⌜persistent_cond P⌝
-                      ∧ rel a p' (λne Wv, P Wv.1 Wv.2)
-                      ∧ ▷ zcond P
-                      ∧ (if readAllowed p' then ▷ rcond P interp else True)
-                      ∧ (if writeAllowed p' then ▷ wcond P interp else True)
-                      ∧ monoReq W a p' P
-                      ∧ ⌜ region_state_nwl W a g ⌝
-              | _ => False
-              end)%I.
-  Solve All Obligations with solve_proper.
-
-  Program Definition interp_cap_RWX (interp : D) : D :=
-    λne W w, (match w with
-              | WCap RWX g b e a =>
-                  [∗ list] a ∈ (finz.seq_between b e),
-                    ∃ (p' : Perm) (P:D),
-                      ⌜PermFlowsTo RWX p'⌝
-                      ∧ ⌜persistent_cond P⌝
-                      ∧ rel a p' (λne Wv, P Wv.1 Wv.2)
-                      ∧ ▷ zcond P
-                      ∧ (if readAllowed p' then ▷ rcond P interp else True)
-                      ∧ (if writeAllowed p' then ▷ wcond P interp else True)
-                      ∧ monoReq W a p' P
-                      ∧ ⌜ region_state_nwl W a g ⌝
-              | _ => False
-              end)%I.
-  Solve All Obligations with solve_proper.
-
-  Program Definition interp_cap_RWLX (interp : D) : D :=
-    λne W w, (match w with
-              | WCap RWLX Local b e a =>
-                  [∗ list] a ∈ (finz.seq_between b e),
-                    ∃ (p' : Perm) (P:D),
-                      ⌜PermFlowsTo RWLX p'⌝
-                      ∧ ⌜persistent_cond P⌝
-                      ∧ rel a p' (λne Wv, P Wv.1 Wv.2)
-                      ∧ ▷ zcond P
-                      ∧ (if readAllowed p' then ▷ rcond P interp else True)
-                      ∧ (if writeAllowed p' then ▷ wcond P interp else True)
-                      ∧ monoReq W a p' P
-                      ∧ ⌜ region_state_pwl W a ⌝
-              | _ => False
-              end)%I.
-  Solve All Obligations with solve_proper.
 
   (* (un)seal permission definitions *)
   (* Note the asymmetry: to seal values, we need to know that we are using a persistent predicate to create a value, whereas we do not need this information when unsealing values (it is provided by the `interp_sb` case). *)
@@ -354,7 +240,8 @@ Program Definition interp_expr (interp : D) r : D :=
     ([∗ list] a ∈ (finz.seq_between b e),
        ∃ P : D,  ⌜∀ w W, Persistent (P W w)⌝ ∗ (∀ W, seal_pred a (P W)) ∗ ▷ wcond P interp)%I.
   Definition safe_to_unseal (interp : D) (b e : OType) : iPropO Σ :=
-    ([∗ list] a ∈ (finz.seq_between b e), ∃ P : D, (∀ W, seal_pred a (P W)) ∗ ▷ rcond P interp)%I.
+    ([∗ list] a ∈ (finz.seq_between b e),
+       ∃ P : D, (∀ W, seal_pred a (P W)) ∗ ▷ rcond RO P interp)%I.
 
   Program Definition interp_sr (interp : D) : D :=
     λne W w, (match w with
@@ -365,27 +252,25 @@ Program Definition interp_expr (interp : D) r : D :=
   Solve All Obligations with solve_proper.
 
   Program Definition interp_sb (o : OType) (w : Word) :=
-    (∃ P : Word → iPropI Σ,  ⌜∀ w, Persistent (P w)⌝ ∗ seal_pred o P ∗ ▷ P w)%I.
+    (∃ P : Word → iPropI Σ,  ⌜∀ w, Persistent (P w)⌝
+                                   ∗ seal_pred o P
+                                   ∗ ▷ P w
+                                   ∗ ▷ P (borrow w)
+    )%I.
+
+  Definition interp_False : D := λne _ _, False%I.
 
   Program Definition interp1 (interp : D) : D :=
     (λne W w,
     match w return _ with
     | WInt _ => interp_z W w
-    | WCap O g b e a => interp_cap_O W w
-    | WCap WO g b e a => interp_cap_WO interp W w
-    | WCap WLO g b e a => interp_cap_WLO interp W w
-    | WCap RO g b e a => interp_cap_RO interp W w
-    | WCap RW g b e a => interp_cap_RW interp W w
-    | WCap RWL g b e a => interp_cap_RWL interp W w
-    | WCap RX g b e a => interp_cap_RX interp W w
-    | WCap RWX g b e a => interp_cap_RWX interp W w
-    | WCap RWLX g b e a => interp_cap_RWLX interp W w
+    | WCap (O _ _) g b e a => interp_cap_O W w
     | WCap E g b e a => interp_cap_E interp W w
+    | WCap _ g b e a => interp_cap interp W w
     | WSealRange p g b e a => interp_sr interp W w
     | WSealed o sb => interp_sb o (WSealable sb)
     end)%I.
   Solve All Obligations with solve_proper.
-
 
   Global Instance interp_cap_O_contractive :
     Contractive (interp_cap_O).
@@ -399,69 +284,15 @@ Program Definition interp_expr (interp : D) r : D :=
     all: solve_contractive.
   Qed.
 
-  Global Instance interp_cap_WO_contractive :
-    Contractive (interp_cap_WO).
+  Global Instance interp_cap_contractive :
+    Contractive (interp_cap).
   Proof.
-    solve_proper_prepare.
-    destruct_word x1; auto.
-    destruct_perm c ; auto ; solve_contractive.
-  Qed.
-
-  Global Instance interp_cap_WLO_contractive :
-    Contractive (interp_cap_WLO).
-  Proof.
-    solve_proper_prepare.
-    destruct_word x1; auto.
-    destruct_perm c ; destruct g ; auto ; solve_contractive.
-  Qed.
-
-  Global Instance interp_cap_RO_contractive :
-    Contractive (interp_cap_RO).
-  Proof.
-    solve_proper_prepare.
-    destruct_word x1; auto.
-    destruct_perm c ; auto ; solve_contractive.
-  Qed.
-
-  Global Instance interp_cap_RW_contractive :
-    Contractive (interp_cap_RW).
-  Proof.
-    solve_proper_prepare.
-    destruct_word x1; auto.
-    destruct_perm c ; auto ; solve_contractive.
-  Qed.
-
-  Global Instance interp_cap_RWL_contractive :
-    Contractive (interp_cap_RWL).
-  Proof.
-    solve_proper_prepare.
-    destruct_word x1; auto.
-    destruct_perm c ; destruct g ; auto ; solve_contractive.
-  Qed.
-
-  Global Instance interp_cap_RX_contractive :
-    Contractive (interp_cap_RX).
-  Proof.
-    solve_proper_prepare.
-    destruct_word x1; auto.
-    destruct_perm c ; auto ; solve_contractive.
-  Qed.
-
-  Global Instance interp_cap_RWX_contractive :
-    Contractive (interp_cap_RWX).
-  Proof.
-    solve_proper_prepare.
-    destruct_word x1; auto.
-    destruct_perm c ; auto ; solve_contractive.
-  Qed.
-
-  Global Instance interp_cap_RWLX_contractive :
-    Contractive (interp_cap_RWLX).
-  Proof.
-    solve_proper_prepare.
-    destruct_word x1; auto.
-    destruct_perm c ; destruct g ; auto ; solve_contractive.
-  Qed.
+    (* solve_proper_prepare. *)
+    (* destruct_word x1; auto. *)
+    (* destruct c ; auto. *)
+    (* destruct rx,w,g; auto. *)
+    (* par: solve_contractive. (* TODO how can I set -async-proofs-tac-j *) *)
+  Admitted. (* TODO holds, but very loooong *)
 
   Global Instance interp_sr_contractive :
     Contractive (interp_sr).
@@ -476,23 +307,17 @@ Program Definition interp_expr (interp : D) r : D :=
   Global Instance interp1_contractive :
     Contractive (interp1).
   Proof.
-    intros n x y Hdistn W w.
-    rewrite /interp1.
-    destruct_word w; [auto|..].
-    + destruct c; first auto ; cycle 1.
-      - by apply interp_cap_E_contractive.
-      - destruct rx,w; first auto.
-        * by apply interp_cap_WO_contractive.
-        * by apply interp_cap_WLO_contractive.
-        * by apply interp_cap_RO_contractive.
-        * by apply interp_cap_RW_contractive.
-        * by apply interp_cap_RWL_contractive.
-        * by apply interp_cap_RX_contractive.
-        * by apply interp_cap_RWX_contractive.
-        * by apply interp_cap_RWLX_contractive.
-   + by apply interp_sr_contractive.
-   + rewrite /interp_sb; solve_contractive.
-  Qed.
+   (*  intros n x y Hdistn W w. *)
+   (*  rewrite /interp1. *)
+   (*  destruct_word w; [auto|..]. *)
+   (*  + destruct c; first auto ; cycle 1. *)
+   (*    - by apply interp_cap_E_contractive. *)
+   (*    - destruct rx,w,dl,dro. *)
+   (*      par: try (by apply interp_cap_O_contractive). *)
+   (*      par: by apply interp_cap_contractive. *)
+   (* + by apply interp_sr_contractive. *)
+   (* + rewrite /interp_sb; solve_contractive. *)
+  Admitted. (* TODO holds, but very loooong *)
 
   Lemma fixpoint_interp1_eq (W : WORLD) (x : leibnizO Word) :
     fixpoint (interp1) W x ≡ interp1 (fixpoint (interp1)) W x.
@@ -504,31 +329,29 @@ Program Definition interp_expr (interp : D) r : D :=
   Definition interp_registers : R := interp_reg interp.
 
   Global Instance interp_persistent W w : Persistent (interp W w).
-  Proof. intros. destruct_word w; simpl; rewrite fixpoint_interp1_eq; simpl.
-         - apply _.
-         - destruct_perm c ; destruct g; repeat (apply exist_persistent; intros); try apply _.
-         - destruct (permit_seal sr), (permit_unseal sr); rewrite /safe_to_seal /safe_to_unseal; apply _ .
-         - apply exist_persistent; intros P.
-           unfold Persistent. iIntros "(Hpers & #Hs & HP)".
-           iDestruct "Hpers" as %Hpers.
-           (* use knowledge about persistence *)
-           iAssert (<pers> ▷ P (WSealable sb))%I with "[ HP ]" as "HP".
-           { iApply later_persistently_1. by iApply Hpers.  }
-           iApply persistently_sep_2; iSplitR; auto.
-           iApply persistently_sep_2; auto.
-  Qed.
+  Proof.
+    (* intros. destruct_word w; simpl; rewrite fixpoint_interp1_eq; simpl. *)
+    (* - apply _. *)
+    (* - destruct_perm c ; destruct g; repeat (apply exist_persistent; intros); try apply _. *)
+    (* - destruct (permit_seal sr), (permit_unseal sr); rewrite /safe_to_seal /safe_to_unseal; apply _ . *)
+    (* - apply exist_persistent; intros P. *)
+    (*   unfold Persistent. iIntros "(Hpers & #Hs & HP & HPborrowed)". *)
+    (*   iDestruct "Hpers" as %Hpers. *)
+    (*   (* use knowledge about persistence *) *)
+    (*   iAssert (<pers> ▷ P (WSealable sb))%I with "[ HP ]" as "HP". *)
+    (*   { iApply later_persistently_1. by iApply Hpers.  } *)
+    (*   iAssert (<pers> ▷ P (borrow (WSealable sb)))%I with "[ HPborrowed ]" as "HPborrowed". *)
+    (*   { iApply later_persistently_1. by iApply Hpers.  } *)
+    (*   iApply persistently_sep_2; iSplitR; auto. *)
+    (*   iApply persistently_sep_2; auto. *)
+  Admitted. (* TODO holds, but very loooong *)
 
   (* Non-curried version of interp *)
   Definition interpC := safeC interp.
 
-  (* TODO readAllow p or p'?
-     On previous version, it was only based on p
-     ; but in my paper, version, it is p'.
-     Which one?
-   *)
   Lemma interp1_eq interp (W: WORLD) p g b e a:
     ((interp1 interp W (WCap p g b e a)) ≡
-       (if (decide (p=O))
+       (if (isO p)
         then True
         else
           if (isSentry p)
@@ -539,44 +362,43 @@ Program Definition interp_expr (interp : D) r : D :=
                     ∗ ⌜persistent_cond P⌝
                     ∗ rel a p' (safeC P)
                     ∗ ▷ zcond P
-                    ∗ (if readAllowed p' then ▷ (rcond P interp) else True)
+                    ∗ (if readAllowed p' then ▷ (rcond p' P interp) else True)
                     ∗ (if writeAllowed p' then ▷ (wcond P interp) else True)
                     ∗ monoReq W a p' P
                     ∗ ⌜ if pwl p then region_state_pwl W a else region_state_nwl W a g⌝)
                ∗ (⌜ if pwl p then g = Local else True⌝))%I).
   Proof.
-    iSplit.
-    { iIntros "HA".
-      destruct (decide (p=O)); subst; auto.
-      destruct (isSentry p) eqn:Hsentry; subst; auto.
-      { destruct p ; cbn in *;auto. congruence. }
-      destruct p; cbn in Hsentry; try congruence; auto ; clear Hsentry.
-      cbn.
-      destruct rx
-      ; destruct w ; try congruence ; auto
-      ; destruct g ;auto
-      ; try (iSplit;eauto).
-      all: try (iApply (big_sepL_mono with "HA"); intros k a' ?; iIntros "H").
-      all: try (iDestruct "H" as (p' P Hflp' Hpers) "(Hrel & Hzcond & Hrcond & Hwcond & HmonoR & %Hstate_a')").
-      all: try (iExists p',P ; iFrame "#∗"; repeat (iSplit;[done|];done)).
-    }
-    { iIntros "A".
-      destruct (decide (p = O)); subst; auto.
-      destruct (isSentry p) eqn:Hsentry; subst; auto.
-      { destruct p ; cbn in *;auto. congruence. }
-      iDestruct "A" as "(A & %)".
-      destruct_perm p; cbn in Hsentry; try congruence; auto ; clear Hsentry.
-      all: destruct g eqn:Hg; simplify_eq ; eauto ; cbn.
-      all: try (iApply (big_sepL_mono with "A"); intros; iIntros "H").
-      all: try (iDestruct "H" as (p' P Hflp' Hpers) "(Hrel & Hzcond & Hrcond & Hwcond & HmonoR & %Hstate_a')").
-      all: try (iExists p',P ; iFrame "#∗"; repeat (iSplit;[done|];done)).
-      all: try (iApply (big_sepL_mono with "A"); intros; iIntros "H").
-    }
-  Qed.
+    (* iSplit. *)
+    (* { iIntros "HA". *)
+    (*   destruct (isO p) eqn:HnotO; subst; auto. *)
+    (*   destruct (isSentry p) eqn:Hsentry; subst; auto. *)
+    (*   { destruct p ; cbn in *;auto; congruence. } *)
+    (*   destruct p; cbn in Hsentry; try congruence; auto ; clear Hsentry. *)
+    (*   cbn. *)
+    (*   destruct rx ; destruct w ; try (cbn in HnotO ; congruence); auto. *)
+    (*   all: destruct g ;auto ; try (iSplit;eauto). *)
+    (*   all: try (iApply (big_sepL_mono with "HA"); intros k a' ?; iIntros "H"). *)
+    (*   all: try (iDestruct "H" as (p' P Hflp' Hpers) "(Hrel & Hzcond & Hrcond & Hwcond & HmonoR & %Hstate_a')"). *)
+    (*   all: try (iExists p',P ; iFrame "#∗"; repeat (iSplit;[done|];done)). *)
+    (* } *)
+    (* { iIntros "A". *)
+    (*   destruct (isO p) eqn:HnotO; subst; auto. *)
+    (*   { destruct_perm p ; cbn in *;auto;try congruence. } *)
+    (*   destruct (isSentry p) eqn:Hsentry; subst; auto. *)
+    (*   { destruct p ; cbn in *;auto;congruence. } *)
 
-  Lemma interp_int W n : ⊢ interp W (WInt n).
-  Proof. iIntros. rewrite /interp fixpoint_interp1_eq //. Qed.
+    (*   iDestruct "A" as "(A & %)". *)
+    (*   destruct_perm p; cbn in HnotO,Hsentry; try congruence; auto ; clear Hsentry. *)
+    (*   all: destruct g eqn:Hg; simplify_eq ; eauto ; cbn. *)
+    (*   all: try (iApply (big_sepL_mono with "A"); intros; iIntros "H"). *)
+    (*   all: try (iDestruct "H" as (p' P Hflp' Hpers) "(Hrel & Hzcond & Hrcond & Hwcond & HmonoR & %Hstate_a')"). *)
+    (*   all: try (iExists p',P ; iFrame "#∗"; repeat (iSplit;[done|];done)). *)
+    (*   all: try (iApply (big_sepL_mono with "A"); intros; iIntros "H"). *)
+    (* } *)
+  Admitted. (* TODO holds, but very long to compile *)
 
+
+  (* Inversion lemmas about interp  *)
   Lemma read_allowed_inv W (a' a b e: Addr) p g :
     (b ≤ a' ∧ a' < e)%Z →
     readAllowed p →
@@ -586,19 +408,25 @@ Program Definition interp_expr (interp : D) r : D :=
       ∗ ⌜persistent_cond P⌝
       ∗ rel a' p' (safeC P)
       ∗ ▷ zcond P
-      ∗ ▷ rcond P interp
+      ∗ ▷ rcond p' P interp
       ∗ (if writeAllowed p' then (▷ wcond P interp) else True)
       ∗ monoReq W a' p' P
   .
   Proof.
     iIntros (Hin Ra) "Hinterp".
-    rewrite /interp. cbn. rewrite fixpoint_interp1_eq /=; cbn.
-    destruct g; try done;cbn.
-    all: destruct_perm p; try done;cbn.
-    all: try (iDestruct (extract_from_region_inv with "Hinterp")
-             as (p P Hfl Hpers) "(Hrel & Hzcond & Hrcond & Hwcond & HmonoR & _)"); eauto.
-    all: try (iExists p,P ; destruct_perm p; iFrame "#∗"; repeat (iSplit;[done|];done)).
-    all: try done.
+    apply Is_true_eq_true in Ra.
+    rewrite /interp. cbn.
+    rewrite fixpoint_interp1_eq interp1_eq; cbn.
+    replace (isO p) with false.
+    2: { eapply readAllowed_nonO in Ra ;done. }
+    replace (isSentry p) with false.
+    2: { eapply readAllowed_isnot_sentry in Ra ;done. }
+    iDestruct "Hinterp" as "[Hinterp %Hloc]".
+    iDestruct (extract_from_region_inv with "Hinterp")
+             as (p' P' Hfl' Hpers') "(Hrel & Hzcond & Hrcond & Hwcond & HmonoR & _)";eauto.
+    pose proof (readAllowed_flows _ _ Hfl' Ra) as Ra'.
+    rewrite Ra'.
+    iExists p',P'; iFrame "#∗%"; try done.
   Qed.
 
 
@@ -612,18 +440,70 @@ Program Definition interp_expr (interp : D) r : D :=
       ∗ rel a' p' (safeC P)
       ∗ ▷ zcond P
       ∗ ▷ wcond P interp
-      ∗ (if readAllowed p' then (▷ rcond P interp) else True)
+      ∗ (if readAllowed p' then (▷ rcond p' P interp) else True)
       ∗ monoReq W a' p' P
   .
   Proof.
     iIntros (Hin Ra) "Hinterp".
-    rewrite /interp. cbn. rewrite fixpoint_interp1_eq /=; cbn.
-    destruct g; try done;cbn.
-    all: destruct_perm p; try done;cbn.
-    all: try (iDestruct (extract_from_region_inv with "Hinterp")
-             as (p P Hfl Hpers) "(Hrel & Hzcond & Hrcond & Hwcond & HmonoR & _)"); eauto.
-    all: try (iExists p,P ; destruct_perm p; iFrame "#∗"; repeat (iSplit;[done|];done)).
-    all: try done.
+    apply Is_true_eq_true in Ra.
+    rewrite /interp. cbn.
+    rewrite fixpoint_interp1_eq interp1_eq; cbn.
+    replace (isO p) with false.
+    2: { eapply writeAllowed_nonO in Ra ;done. }
+    replace (isSentry p) with false.
+    2: { eapply writeAllowed_isnot_sentry in Ra ;done. }
+    iDestruct "Hinterp" as "[Hinterp %Hloc]".
+    iDestruct (extract_from_region_inv with "Hinterp")
+             as (p' P' Hfl' Hpers') "(Hrel & Hzcond & Hrcond & Hwcond & HmonoR & _)";eauto.
+    pose proof (writeAllowed_flows _ _ Hfl' Ra) as Ra'.
+    rewrite Ra'.
+    iExists p',P'; iFrame "#∗%"; try done.
+  Qed.
+
+  Lemma readAllowed_valid_cap_implies W p g b e a:
+    readAllowed p = true ->
+    withinBounds b e a = true ->
+    interp W (WCap p g b e a) -∗
+           ⌜∃ ρ, std W !! a = Some ρ ∧ ρ <> Revoked ∧ (∀ m, ρ ≠ Frozen m)⌝.
+  Proof.
+    intros Hra Hb. iIntros "Hinterp".
+    eapply withinBounds_le_addr in Hb.
+    rewrite /interp. cbn.
+    rewrite fixpoint_interp1_eq interp1_eq; cbn.
+    replace (isO p) with false.
+    2: { eapply readAllowed_nonO in Hra ;done. }
+    replace (isSentry p) with false.
+    2: { eapply readAllowed_isnot_sentry in Hra ;done. }
+    iDestruct "Hinterp" as "[Hinterp %Hloc]".
+    iDestruct (extract_from_region_inv with "Hinterp")
+             as (p' P' Hfl' Hpers') "(Hrel & Hzcond & Hrcond & Hwcond & HmonoR & %Hstate)";eauto.
+    iPureIntro.
+    destruct (pwl p); simplify_eq.
+    naive_solver.
+    destruct g; naive_solver.
+  Qed.
+
+  Lemma writeAllowed_valid_cap_implies W p g b e a:
+    writeAllowed p = true ->
+    withinBounds b e a = true ->
+    interp W (WCap p g b e a) -∗
+           ⌜∃ ρ, std W !! a = Some ρ ∧ ρ <> Revoked ∧ (∀ m, ρ ≠ Frozen m)⌝.
+  Proof.
+    intros Hra Hb. iIntros "Hinterp".
+    eapply withinBounds_le_addr in Hb.
+    rewrite /interp. cbn.
+    rewrite fixpoint_interp1_eq interp1_eq; cbn.
+    replace (isO p) with false.
+    2: { eapply writeAllowed_nonO in Hra ;done. }
+    replace (isSentry p) with false.
+    2: { eapply writeAllowed_isnot_sentry in Hra ;done. }
+    iDestruct "Hinterp" as "[Hinterp %Hloc]".
+    iDestruct (extract_from_region_inv with "Hinterp")
+             as (p' P' Hfl' Hpers') "(Hrel & Hzcond & Hrcond & Hwcond & HmonoR & %Hstate)";eauto.
+    iPureIntro.
+    destruct (pwl p); simplify_eq.
+    naive_solver.
+    destruct g; naive_solver.
   Qed.
 
   Lemma writeLocalAllowed_implies_local W p g b e a:
@@ -635,142 +515,34 @@ Program Definition interp_expr (interp : D) r : D :=
     destruct_perm p; simpl in H; try congruence; destruct g; auto.
   Qed.
 
-  Lemma readAllowed_valid_cap_implies W p g b e a:
-    readAllowed p = true ->
+  Lemma writeLocalAllowed_valid_cap_implies W p g b e a:
+    pwl p = true ->
     withinBounds b e a = true ->
     interp W (WCap p g b e a) -∗
-           ⌜∃ ρ, std W !! a = Some ρ ∧ ρ <> Revoked ∧ (∀ m, ρ ≠ Frozen m)⌝.
+           ⌜std W !! a = Some Temporary⌝.
   Proof.
-    intros Hp Hb. iIntros "H".
+    intros Hp Hb. iIntros "Hinterp".
     eapply withinBounds_le_addr in Hb.
-    unfold interp; rewrite fixpoint_interp1_eq /=.
-    destruct_perm p; simpl in Hp; try congruence.
-    all: try (iDestruct (extract_from_region_inv with "H")
-             as (p P Hfl Hpers) "(Hrel & Hzcond & Hrcond & Hwcond & HmonoR & %Hstate)"); eauto.
-    all: try (destruct g ; auto;
-             iDestruct (extract_from_region_inv with "H")
-             as (p P Hfl Hpers) "(Hrel & Hzcond & Hrcond & Hwcond & HmonoR & %Hstate)"); eauto.
-    all: iPureIntro.
-    all: try (destruct g; eauto;simpl in Hstate; destruct Hstate as [Hstate|Hstate]; eauto).
+    rewrite fixpoint_interp1_eq interp1_eq; cbn.
+    replace (isO p) with false.
+    2: { eapply pwl_nonO in Hp ;done. }
+    replace (isSentry p) with false.
+    2: { eapply pwl_isnot_sentry in Hp ;done. }
+    iDestruct "Hinterp" as "[Hinterp %Hloc]".
+    iDestruct (extract_from_region_inv with "Hinterp")
+             as (p' P' Hfl' Hpers') "(Hrel & Hzcond & Hrcond & Hwcond & HmonoR & %Hstate)";eauto.
+    by rewrite Hp in Hstate.
   Qed.
 
-  Lemma writeAllowed_valid_cap_implies W p g b e a:
-    writeAllowed p = true ->
-    withinBounds b e a = true ->
-    interp W (WCap p g b e a) -∗
-           ⌜∃ ρ, std W !! a = Some ρ ∧ ρ <> Revoked ∧ (∀ m, ρ ≠ Frozen m)⌝.
-  Proof.
-    intros Hp Hb. iIntros "H".
-    eapply withinBounds_le_addr in Hb.
-    unfold interp; rewrite fixpoint_interp1_eq /=.
-    destruct_perm p; simpl in Hp; try congruence.
-    (* all: try (iDestruct (extract_from_region_inv with "H") *)
-    (*          as (p P Hfl Hpers) "(Hrel & Hzcond & Hrcond & %Hstate)"); eauto. *)
-    all: try (iDestruct (extract_from_region_inv with "H")
-             as (p P Hfl Hpers) "(Hrel & Hzcond & Hrcond & Hwcond & HmonoR & %Hstate)"); eauto.
-    all: try (destruct g ; auto;
-             iDestruct (extract_from_region_inv with "H")
-             as (p P Hfl Hpers) "(Hrel & Hzcond & Hrcond & Hwcond & HmonoR & %Hstate)"); eauto.
-    (* all: try (destruct g ; auto; *)
-    (*          iDestruct (extract_from_region_inv with "H") *)
-    (*          as (p P Hfl Hpers) "(Hrel & Hzcond & Hwcond & %Hstate)"); eauto. *)
-    all: iPureIntro.
-    all: try (destruct g; eauto;simpl in Hstate; destruct Hstate as [Hstate|Hstate]; eauto).
-  Qed.
-
-  Lemma persistent_cond_interp : persistent_cond interp.
-  Proof.
-    intros W; apply _.
-  Qed.
-
-  Lemma zcond_interp : ⊢ zcond interp.
-  Proof.
-    by iModIntro; iIntros (W1 W2 w) "_"; iApply interp_int.
-  Qed.
-
-  Lemma rcond_interp : ⊢ rcond interp interp.
-  Proof.
-    by iModIntro; iIntros (W1 w) "?".
-  Qed.
-
-  Lemma wcond_interp : ⊢ wcond interp interp.
-  Proof.
-    by iModIntro; iIntros (W1 w) "?".
-  Qed.
-
-  (* Lemma read_allowed_inv_regs (a' a b e: Addr) p g W r : *)
-  (*   (b ≤ a' ∧ a' < e)%Z → *)
-  (*   readAllowed p → *)
-  (*   ⊢ (interp_registers W r -∗ *)
-  (*     interp W (WCap p g b e a) -∗ *)
-  (*     (∃ (p' : Perm) (P : D), *)
-  (*         ⌜persistent_cond P⌝ *)
-  (*         ∗ rel a' p' (λ Wv, P Wv.1 Wv.2) *)
-  (*         ∗ ▷ zcond P *)
-  (*         ∗ (if decide (readAllowed_in_r_a (<[PC:=(WCap p g b e a)]> r) a') *)
-  (*           then ▷ rcond P interp *)
-  (*           else emp) *)
-  (*         ∗ (if decide (writeAllowed_in_r_a (<[PC:=(WCap p g b e a)]> r) a') *)
-  (*           then ▷ wcond P interp *)
-  (*           else emp)))%I. *)
-  (* Proof. *)
-  (*   iIntros (Hin Ra) "#Hregs #Hinterp". *)
-  (*   rewrite /interp_registers /interp_reg /=. *)
-  (*   iDestruct "Hregs" as "[Hfull Hregvalid]". *)
-  (*   case_decide as Hinra. *)
-  (*   - destruct Hinra as [reg (wa & Hra & Hwa & Ha) ]. *)
-  (*     destruct (decide (reg = PC)). *)
-  (*     + simplify_map_eq. *)
-  (*       rewrite fixpoint_interp1_eq /=; cbn. *)
-  (*       destruct_perm p *)
-  (*       ; destruct g *)
-  (*       ; try contradiction ; try done *)
-  (*       ; inversion Hwa; try done. *)
-  (*       all: try (iDestruct (extract_from_region_inv with "Hinterp") *)
-  (*         as (p P Hfl Hpers) "(Hrel & Hzcond & Hrcond & Hwcond & %Hstate)" *)
-  (*       ; eauto ; iClear "Hinterp Hregvalid"). *)
-  (*       all: try (iDestruct (extract_from_region_inv with "Hinterp") *)
-  (*         as (p P Hfl Hpers) "(Hrel & Hzcond & Hcond & %Hstate)" *)
-  (*       ; eauto ; iClear "Hinterp Hregvalid"). *)
-  (*       all: try (iExists p,P; iFrame "#"; done). *)
-  (*     + simplify_map_eq. *)
-  (*       destruct wa; try inv Ha. *)
-  (*       destruct sb; try inv Ha. *)
-  (*       iSpecialize ("Hregvalid" $! _ _ n Hra). *)
-  (*       iClear "Hinterp". *)
-  (*       rewrite fixpoint_interp1_eq /=; cbn. *)
-  (*       destruct_perm p0 *)
-  (*       ; cbn in Hwa *)
-  (*       ; destruct g0 *)
-  (*       ; try contradiction; inversion Hwa; try done ; subst. *)
-  (*       all: try (iDestruct (extract_from_region_inv with "Hregvalid") *)
-  (*         as (p' P' Hfl' Hpers') "(Hrel & Hzcond & Hrcond & Hwcond & %Hstate)" *)
-  (*       ; eauto ; iClear "Hregvalid"). *)
-  (*       all: try (iDestruct (extract_from_region_inv with "Hregvalid") *)
-  (*         as (p' P' Hfl' Hpers') "(Hrel & Hzcond & Hwcond & %Hstate)" *)
-  (*       ; eauto ; iClear "Hregvalid"). *)
-  (*       all: iExists p',P'; iFrame "#"; done. *)
-  (*   - rewrite fixpoint_interp1_eq /=; cbn. *)
-  (*     destruct p,g; try contradiction; try done. *)
-  (*     all: try (iDestruct (extract_from_region_inv with "Hinterp") *)
-  (*              as (p P Hfl Hpers) "(Hrel & Hzcond & Hrcond & %Hstate)" *)
-  (*               ; eauto ; iClear "Hinterp Hregvalid"). *)
-  (*     all: try (iDestruct (extract_from_region_inv with "Hinterp") *)
-  (*              as (p P Hfl Hpers) "(Hrel & Hzcond & Hrcond & Hwcond & %Hstate)" *)
-  (*               ; eauto ; iClear "Hinterp Hregvalid"). *)
-  (*     all: iExists p,P; iFrame "#"; done. *)
-  (* Qed. *)
-
-  Lemma write_allowed_implies_ra
+  Lemma interp_in_registers
     W (regs : leibnizO Reg) (p : Perm) (g : Locality) (b e a : Addr):
-    readAllowed p = true
-    -> (∀ (r : RegName) (v : Word), ⌜r ≠ PC⌝ → ⌜regs !! r = Some v⌝ → fixpoint interp1 W v)%I
+      (∀ (r : RegName) (v : Word), ⌜r ≠ PC⌝ → ⌜regs !! r = Some v⌝ → fixpoint interp1 W v)%I
     -∗ (∃ (p' : Perm) (P : D),
         ⌜PermFlowsTo p p'⌝
         ∗ ⌜persistent_cond P⌝
         ∗ rel a p' (safeC P)
         ∗ ▷ zcond P
-        ∗ (if readAllowed p' then ▷ rcond P interp else True)
+        ∗ (if readAllowed p' then ▷ rcond p' P interp else True)
         ∗ (if writeAllowed p' then ▷ wcond P interp else True)
         ∗ monoReq W a p' P
         ∗ ⌜if pwl p then region_state_pwl W a else region_state_nwl W a g⌝
@@ -780,7 +552,9 @@ Program Definition interp_expr (interp : D) r : D :=
         ∗ ⌜persistent_cond P⌝
         ∗ rel a p' (safeC P)
         ∗ ▷ zcond P
-        ∗ ▷ rcond P interp
+        ∗ (if decide (readAllowed_in_r_a (<[PC:=WCap p g b e a]> regs) a)
+            then ▷ (rcond p' P interp)
+            else emp)
         ∗ (if decide (writeAllowed_in_r_a (<[PC:=WCap p g b e a]> regs) a)
             then ▷ wcond P interp
             else emp)
@@ -788,31 +562,19 @@ Program Definition interp_expr (interp : D) r : D :=
         ∗ ⌜if pwl p then region_state_pwl W a else region_state_nwl W a g⌝
        ).
   Proof.
-    intros Hrap.
     iIntros "#Hreg #H".
     iDestruct "H" as (p0 P0 Hflp0 Hperscond_P0) "(Hrel0 & Hzcond0 & Hrcond0 & Hwcond0 & HmonoR0 & %Hstate0)".
-    destruct (readAllowed p0) eqn:Hrap'; cycle 1.
-    { apply readAllowed_flows in Hflp0; auto; congruence.  }
-    destruct (writeAllowed p0) eqn:Hwa.
-    - iExists p0,P0.
-      iSplit; first (iPureIntro ; apply Hflp0).
-      iSplit; first (iPureIntro ; apply Hperscond_P0).
-      iFrame "#".
-      case_decide;auto.
-    - assert (writeAllowed p = false) as Hwaw'.
-      { destruct_perm p ; destruct_perm p0 ; cbn in * ; try done. }
-      destruct (decide (writeAllowed_in_r_a (<[PC:=WCap p g b e a]> regs) a))
-        as [Hwa'|Hwa']; cycle 1.
-      { iExists p0, P0.
-        iSplit; first (iPureIntro ; apply Hflp0).
-        iSplit; first (iPureIntro ; apply Hperscond_P0).
-        iFrame "#".
-        auto.
-      }
-
-      destruct Hwa' as (r & w & Hsome & Hwaw & Hvw).
+    iExists p0,P0.
+    iFrame "%#".
+    iSplit.
+    - (* rcond *)
+      destruct (decide (readAllowed_in_r_a (<[PC:=WCap p g b e a]> regs) a))
+        as [Hra'|Hra']; auto.
+      destruct (readAllowed p0) eqn:Hra; auto.
+      destruct Hra' as (r & w & Hsome & Hrar & Hvw).
       destruct (decide (r = PC)); subst.
       { rewrite lookup_insert in Hsome; simplify_eq.
+        eapply readAllowed_flows in Hrar; eauto.
         cbn in *; congruence.
       }
       rewrite lookup_insert_ne in Hsome; auto.
@@ -820,8 +582,36 @@ Program Definition interp_expr (interp : D) r : D :=
       destruct_word w; cbn in * ; try done.
       destruct Hvw as [Hvw ->].
       iEval (rewrite fixpoint_interp1_eq interp1_eq) in "Hinterp_w".
-      destruct (decide (c = O)); first (subst; cbn in *;done).
-      destruct (isSentry c) eqn:Henstry ; first (destruct_perm c; cbn in *; try done).
+      replace (isO c) with false.
+      2: { eapply readAllowed_nonO in Hrar ;done. }
+      replace (isSentry c) with false.
+      2: { eapply readAllowed_isnot_sentry in Hrar ;done. }
+      iDestruct "Hinterp_w" as "[Hinterp_w %Hc_cond ]".
+      iDestruct (extract_from_region_inv with "Hinterp_w")
+        as (p1 P1 Hflc1 Hperscond_P1) "(Hrel1 & Hzcond1 & Hrcond1 & Hwcond1 & HmonoR1 & %Hstate1)"
+      ; eauto; iClear "Hinterp_w".
+      apply readAllowed_flows in Hflc1; auto.
+      iDestruct (rel_agree a0 _ _ p0 p1 with "[$Hrel0 $Hrel1]") as "(-> & Heq)".
+      congruence.
+    - (* wcond *)
+      destruct (decide (writeAllowed_in_r_a (<[PC:=WCap p g b e a]> regs) a))
+        as [Hwa'|Hwa']; auto.
+      destruct (writeAllowed p0) eqn:Hwa; auto.
+      destruct Hwa' as (r & w & Hsome & Hwaw & Hvw).
+      destruct (decide (r = PC)); subst.
+      { rewrite lookup_insert in Hsome; simplify_eq.
+        eapply writeAllowed_flows in Hwaw; eauto.
+        cbn in *; congruence.
+      }
+      rewrite lookup_insert_ne in Hsome; auto.
+      iDestruct ("Hreg" $! r w n Hsome) as "Hinterp_w".
+      destruct_word w; cbn in * ; try done.
+      destruct Hvw as [Hvw ->].
+      iEval (rewrite fixpoint_interp1_eq interp1_eq) in "Hinterp_w".
+      replace (isO c) with false.
+      2: { eapply writeAllowed_nonO in Hwaw ;done. }
+      replace (isSentry c) with false.
+      2: { eapply writeAllowed_isnot_sentry in Hwaw ;done. }
       iDestruct "Hinterp_w" as "[Hinterp_w %Hc_cond ]".
       iDestruct (extract_from_region_inv with "Hinterp_w")
         as (p1 P1 Hflc1 Hperscond_P1) "(Hrel1 & Hzcond1 & Hrcond1 & Hwcond1 & HmonoR1 & %Hstate1)"
@@ -830,77 +620,5 @@ Program Definition interp_expr (interp : D) r : D :=
       iDestruct (rel_agree a0 _ _ p0 p1 with "[$Hrel0 $Hrel1]") as "(-> & Heq)".
       congruence.
   Qed.
-
-  Lemma writeLocalAllowed_valid_cap_implies W p g b e a:
-    pwl p = true ->
-    withinBounds b e a = true ->
-    interp W (WCap p g b e a) -∗
-           ⌜std W !! a = Some Temporary⌝.
-  Proof.
-    intros Hp Hb. iIntros "Hvalid".
-    eapply withinBounds_le_addr in Hb.
-    unfold interp; rewrite fixpoint_interp1_eq /=.
-    destruct_perm p; simpl in Hp; try congruence; destruct g;try done.
-    all:try (iDestruct (extract_from_region_inv with "Hvalid") as (????) "(_&_&_&_&_&%)"; eauto).
-  Qed.
-
-  Lemma region_seal_pred_interp E W (b e a: OType) b1 b2 g :
-    ([∗ list] o ∈ finz.seq_between b e, (∀ W, seal_pred o (interp W))) ={E}=∗
-    interp W (WSealRange (b1,b2) g b e a).
-  Proof.
-    remember (finz.seq_between b e) as l eqn:Hgen. rewrite Hgen; revert Hgen.
-    generalize b e. clear b e.
-    induction l as [|hd tl IH].
-    - iIntros (b e Hfinz) "_ !>".
-      rewrite /interp fixpoint_interp1_eq /= /safe_to_seal /safe_to_unseal.
-      rewrite -Hfinz. destruct b1, b2; iSplit; done.
-    - iIntros (b e Hfinz).
-      assert (b < e)%ot as Hlbe.
-      {destruct (decide (b < e)%ot) as [|HF]; first auto. rewrite finz_seq_between_empty in Hfinz; [inversion Hfinz | solve_addr  ]. }
-      apply finz_cons_tl in Hfinz as (b' & Hplus & Hfinz).
-      specialize (IH b' e Hfinz). rewrite (finz_seq_between_split _ b' _).
-      2 : split; solve_addr.
-      iIntros "[#Hfirst Hca]".
-      iMod (IH with "Hca") as "Hca". iModIntro.
-      rewrite /interp !fixpoint_interp1_eq /= /safe_to_seal /safe_to_unseal.
-      rewrite !(finz_seq_between_split b b' e). 2: { split ; solve_addr. }
-      iDestruct "Hca" as "[Hseal Hunseal]".
-      iSplitL "Hseal"; [destruct b1| destruct b2]; iFrame.
-      all: iApply (big_sepL_mono with "Hfirst").
-      all: iIntros (k a' Hk) "H"; cbn.
-      all: iExists _; iFrame; auto.
-      iSplit;first (iPureIntro; apply _).
-      iApply wcond_interp.
-      iApply rcond_interp.
-  Qed.
-
-  (* Lemma monotonicity_guarantees_region_canStore *)
-  (*   (p : Perm) (w : Word) (P : D) *)
-  (*   (ρ : region_type) : *)
-  (*   canStore p w = true *)
-  (*   -> monotonicity_guarantees_regionFull ρ p (safeC P) *)
-  (*     -∗ monotonicity_guarantees_region ρ w p (safeC P). *)
-  (* Proof. *)
-  (*   iIntros (HcanStore) "Hmono". *)
-  (*   destruct ρ; auto; cbn; [destruct (pwl p)|]. *)
-  (*   all: iApply "Hmono"; auto. *)
-  (* Qed. *)
-
-
-  (* Get the validity of sealing capabilities if we can allocate an arbitrary predicate,
-     and can hence choose interp itself as the sealing predicate *)
-  (* Lemma region_can_alloc_interp E W (b e a: OType) b1 b2 g: *)
-  (*   ([∗ list] o ∈ finz.seq_between b e, can_alloc_pred o) ={E}=∗ *)
-  (*   interp W (WSealRange (b1,b2) g b e a). *)
-  (* Proof. *)
-  (*   iIntros "Hca". *)
-  (*   iDestruct (big_sepL_mono with "Hca") as "Hca". *)
-  (*   iIntros (k a' Hk) "H". iDestruct (seal_store_update_alloc _ (interp W)  with "H") as "H". iExact "H". *)
-
-  (*   iDestruct (big_sepL_bupd with "Hca") as "Hca". *)
-  (*   iMod "Hca". *)
-  (*   by iApply region_seal_pred_interp. *)
-  (* Qed. *)
-
 
 End logrel.
