theories/proofmode/solve_pure.v
@@ -37,7 +37,8 @@ Qed.
 
 #[export] Hint Mode isCorrectPC + : solve_pure.
 
-#[export] Hint Resolve isCorrectPC_ExecPCPerm_InBounds : solve_pure.
+#[export] Hint Resolve isCorrectPC_executeAllowed_InBounds : solve_pure.
+(* #[export] Hint Resolve isCorrectPC_ExecPCPerm_InBounds : solve_pure. *)
 
 (* Proxy lemma for DecodeInstr *)
 
@@ -51,22 +52,29 @@ Qed.
 
 (* ExecPCPerm, PermFlowsTo *)
 
-#[export] Hint Mode ExecPCPerm + : solve_pure.
+(* #[export] Hint Mode ExecPCPerm + : solve_pure. *)
 #[export] Hint Mode PermFlowsTo - + : solve_pure.
 
-Lemma ExecPCPerm_InCtx p :
-  InCtx (ExecPCPerm p) → ExecPCPerm p.
-Proof. auto. Qed.
-#[export] Hint Resolve ExecPCPerm_InCtx : solve_pure.
+(* Lemma ExecPCPerm_InCtx p : *)
+(*   InCtx (ExecPCPerm p) → ExecPCPerm p. *)
+(* Proof. auto. Qed. *)
+(* #[export] Hint Resolve ExecPCPerm_InCtx : solve_pure. *)
 
-#[export] Hint Resolve ExecPCPerm_RX : solve_pure.
-#[export] Hint Resolve ExecPCPerm_RWX : solve_pure.
-#[export] Hint Resolve ExecPCPerm_not_E : solve_pure.
-#[export] Hint Resolve ExecPCPerm_flows_to : solve_pure.
+
+Lemma executeAllowed_InCtx p :
+  InCtx (executeAllowed p = true) → (executeAllowed p = true).
+Proof. auto. Qed.
+#[export] Hint Resolve executeAllowed_InCtx : solve_pure.
+
+(* #[export] Hint Resolve ExecPCPerm_RX : solve_pure. *)
+(* #[export] Hint Resolve ExecPCPerm_RWX : solve_pure. *)
+(* #[export] Hint Resolve ExecPCPerm_not_E : solve_pure. *)
+(* #[export] Hint Resolve ExecPCPerm_flows_to : solve_pure. *)
 (* TODO: add a test checking the use of ExecPCPerm_flows_to (if it is still *)
 (*    needed) *)
-#[export] Hint Resolve ExecPCPerm_readAllowed : solve_pure.
+(* #[export] Hint Resolve ExecPCPerm_readAllowed : solve_pure. *)
 (* Will only work if arguments are concrete terms *)
+#[export] Hint Extern 1 (executeAllowed _ = true) => reflexivity : solve_pure.
 #[export] Hint Extern 1 (readAllowed _ = true) => reflexivity : solve_pure.
 #[export] Hint Extern 1 (writeAllowed _ = true) => reflexivity : solve_pure.
 #[export] Hint Extern 1 (PermFlowsTo _ _ = true) => reflexivity : solve_pure.
@@ -105,7 +113,7 @@ Proof. auto. Qed.
 #[export] Hint Extern 1 (is_z _ = true) => reflexivity : solve_pure.
 
 (* isSentry *)
-#[export] Hint Extern 1 (isSentry (BPerm _ _) = false) => done : solve_pure.
+#[export] Hint Extern 1 (isSentry (BPerm _ _ _ _) = false) => done : solve_pure.
 #[export] Hint Extern 1 (isSentry E = true) => done : solve_pure.
 
 (* canStore *)
@@ -132,7 +140,7 @@ Goal forall (r_t1 PC: RegName) `{MachineParameters}, exists r1 r2,
 Proof. do 2 eexists. repeat apply conj. solve_pure. all: reflexivity. Qed.
 
 Goal forall p g b e a,
-  ExecPCPerm p →
+  executeAllowed p = true →
   SubBounds b e a (a ^+ 5)%a →
   ContiguousRegion a 5 →
   isCorrectPC (WCap p g b e a).
@@ -144,7 +152,7 @@ Goal forall (r_t1 r_t2: RegName), exists r1 r2,
 Proof. do 2 eexists. repeat apply conj. solve_pure. all: reflexivity. Qed.
 
 Goal forall p g b e a,
-  ExecPCPerm p →
+  executeAllowed p = true →
   SubBounds b e a (a ^+ 5)%a →
   ContiguousRegion a 5 →
   isCorrectPC (WCap p g b e (a ^+ 1)%a).
